%!TEX root = main.tex
\section{Proofs in \mysec{application}} \label{sec:appapp}
Here we provide further discussion and proofs of results described in \mysec{application}.
\subsection{Proofs in \mysec{geostrong}}
Here we present the proofs of the slow convergence rate (both in 2nd and 4th moments) for SGD applied to geodesically-smooth and strongly-convex functions. As discussed
in \mysec{geostrong} we will take the retraction $R$ to be the exponential map throughout this section.
Before we begin, we recall the following Lemma from \citet{moulines2011non},
 \begin{lemma}\label{lem:computsum} Let $n,m\in\mathbb{N}$ such that $m<n$ and $\alpha\geq0$. Then,
\[
\frac{1}{2(1-\alpha)}[n^{1-\alpha}-m^{1-\alpha}]\leq \sum_{k=m+1}^n n^{-\alpha}\leq \frac{1}{1-\alpha}[n^{1-\alpha}-m^{1-\alpha}].
\]
\end{lemma}
This follows by simply bounding sums via integrals.

With this result we can now show that SGD applied to (local) geodesically-smooth and strongly-convex functions will converge at the ``slow'' rate
with an appropriately decaying size.
\begin{proposition}\label{prop:mom2}
Let Assumptions \ref{assump:manifold}, \ref{assump:noiseunbiased},  \ref{assump:noiseLip} and \ref{assump:strongconv}
  hold for the iterates evolving in  \eq{grad_desc}. Recalling that $\gamma_n=Cn^{-\alpha}$ where $C>0$ and $\alpha\in[1/2,1)$ we have,
\[
\E[d^2(x_{n},x_\star)]\leq \frac{2C  \zeta \upsilon^2}{\mu n^\alpha } + O( \exp(-c\mu n^{1-\alpha} )),
\]
and
\[
\E[d^4(x_{n},x_\star)]\leq\frac{4C(3+\zeta)\zeta\upsilon^4}{\mu n^{2\alpha} } + O( \exp(-c\mu n^{1-\alpha} )).
\]
for some $c > 0$, where $\zeta > 0$ is a constant depending on the geometry of $\M$.
\end{proposition}
\begin{proof}
Throughout we will use $c$ to denote a global, positive constant that may change from line to line. The quantity $\zeta \equiv \zeta(\kappa, c) = \frac{\sqrt{\abs{\kappa}} c}{\tanh(\sqrt{\abs{\kappa}} c)}$ is a geometric quantity from \citet{zhang2016first}, where $\kappa$ denotes the sectional curvature of the manifold.  Note that bound on the sectional curvature is subsumed by Assumption \ref{assump:manifold} -- since it is a smooth function on $\X$, so is bounded.

\paragraph{Bound on the second moment.}
We first prove the 2nd-moment bound by following the proof of Theorem 2 by \citet{moulines2011non}, but adapting it to the setting of g-strong convexity.
Using Corollary 8 (a generalization of the law of cosines to the manifold setting) by \citet{zhang2016first} we have
\begin{equation}\label{eq:mom2}
d^2(x_{n+1},x_\star) \leq d^2(x_{n},x_\star) +2\gamma_{n+1}\langle \nabla f_{n+1}(x_n),\Exp_{x_n}^{-1}(x_\star)\rangle +\gamma_{n+1}^2 \zeta \Vert  \nabla f_{n+1}(x_n) \Vert^2,
\end{equation}
where $\zeta$ satisfies $\max_{x\in\X} \zeta(\kappa, d(x,x_\star))\leq \zeta$.
Taking conditional expectations yields
\[
\E[d^2(x_{n+1},x_\star)\vert \F_n]\leq d^2(x_{n},x_\star) +2\gamma_{n+1}\langle \nabla f(x_n),\Exp_{x_n}^{-1}(x_\star)\rangle +\gamma_{n+1}^2 \zeta  \E[\Vert  \nabla f_{n+1}(x_n) \Vert^2\vert \F_n].
\]
Using the definition of g-strong convexity and Assumptions~\ref{assump:noiseLip},\ref{assump:strongconv} we directly get
 \[
\E[d^2(x_{n+1},x_\star) | \F_n]\leq (1-2\gamma_{n+1}\mu )d^2(x_{n},x_\star)+ \gamma_{n+1}^2 \zeta \upsilon^2.
\]
Taking the full expectation, and denoting by $\delta_{n}=\E[d^2(x_{n},x_\star)]$, we obtain the recursion,
\[
\delta_n\leq (1-2\gamma_{n}\mu )\delta_{n-1}+ \gamma_{n}^2 \zeta \upsilon^2.
\]
Unrolling the recursion we have,
\[
\delta_n\leq \prod_{i=1}^n(1-2\gamma_{i}\mu )\delta_0 + \zeta\upsilon^2 \sum_{i=1}^n \gamma_i^2 \prod_{k=i+1}^n(1-2\mu\gamma_k).
\]
Using the elementary inequality $(1-x)\leq \exp(-x)$ for $x\in\mathbb R$, we observe the first term on the right side decreases exponentially fast. To analyze the second term, we split it into two components around $\lfloor n/2 \rfloor$:
\begin{equation}
\sum_{i=1}^n \gamma_i^2 \prod_{k=i+1}^n(1-2\mu\gamma_k)
=
 \sum_{i=1}^{\lfloor n/2 \rfloor} \gamma_i^2 \prod_{k=i+1}^n(1-2\mu\gamma_k)
 +\sum_{i={\lfloor n/2 \rfloor}+1}^n \gamma_i^2 \prod_{k=i+1}^n(1-2\mu\gamma_k). \label{eq:split}
\end{equation}
For the first term in \eq{split}, using again $(1-x)\leq \exp(-x)$ for $x\in\mathbb R$
\BEAS
 \sum_{i=1}^{\lfloor n/2 \rfloor} \gamma_i^2 \prod_{k=i+1}^n(1-2\mu\gamma_k)
 &\leq&
 \prod_{k=\lfloor n/2 \rfloor+1}^n(1-2\mu\gamma_k)  \sum_{i=1}^{\lfloor n/2 \rfloor} \gamma_i^2\\
  &\leq&
 \prod_{k=\lfloor n/2 \rfloor+1}^n\exp(-2\mu\gamma_k)  \sum_{i=1}^{\lfloor n/2 \rfloor} \gamma_i^2\\
  &\leq&
 \exp(-2\mu \sum_{k=\lfloor n/2 \rfloor+1}^n\gamma_k)  \sum_{i=1}^{\lfloor n/2 \rfloor} \gamma_i^2\\
   &\leq&
 C \exp(-{c\mu }n^{1-\alpha}) n^{1-2\alpha},
\EEAS
using Lemma \ref{lem:computsum}, which will decrease exponentially fast as $n \to \infty$. For the second term,
\BEAS
\sum_{i={\lfloor n/2 \rfloor}+1}^n \gamma_i^2 \prod_{k=i+1}^n(1-\mu\gamma_k)&\leq&\gamma_{\lfloor n/2 \rfloor}\sum_{i={\lfloor n/2 \rfloor}+1}^n \gamma_i \prod_{k=i+1}^n(1-\mu\gamma_k)\\
&=&\gamma_{\lfloor n/2 \rfloor}\sum_{i={\lfloor n/2 \rfloor}+1}^n\frac{ 1-(1-\mu\gamma_i)}{\mu} \prod_{k=i+1}^n(1-\mu\gamma_k) \\
&=&\frac{\gamma_{\lfloor n/2 \rfloor}}{\mu}\sum_{i={\lfloor n/2 \rfloor}+1}^n [ \prod_{k=i+1}^n(1-\mu\gamma_k)-\prod_{k=i}^n(1-\mu\gamma_k)]\\
&\leq&\frac{\gamma_{\lfloor n/2 \rfloor}}{\mu}[1-\prod_{k=\lfloor n/2 \rfloor+2}^n(1-\mu\gamma_k)]]\\
&\leq&\frac{\gamma_{\lfloor n/2 \rfloor}}{\mu}\leq \frac{2C}{n^\alpha\mu}.
\EEAS
The bound on the second moment follows from this last inequality.
\paragraph{Bound on the fourth moment.}
We now prove the bound on the 4th-moment. We start by expanding the square of \eq{mom2},
\begin{multline*}
d^4(x_{n+1},x_\star) \leq d^4(x_{n},x_\star) +4\gamma_{n+1}^2(\langle \nabla f_{n+1}(x_n),\Exp_{x_n}^{-1}(x_\star)\rangle)^2 +\gamma_{n+1}^4 \zeta^2 \Vert  \nabla f_{n+1}(x_n) \Vert^4 \\ +4 \gamma_{n+1}\langle \nabla f_{n+1}(x_n),\Exp_{x_n}^{-1}(x_\star)\rangle d^2(x_{n},x_\star)  +2 \gamma_{n+1}^2 \zeta \Vert  \nabla f_{n+1}(x_n) \Vert^2d^2(x_{n},x_\star) \\+ 4 \gamma_{n+1}^3\langle \nabla f_{n+1}(x_n),\Exp_{x_n}^{-1}(x_\star)\rangle \zeta \Vert  \nabla f_{n+1}(x_n) \Vert^2.
\end{multline*}
Taking conditional expectations and using Cauchy-Schwarz we have,
\BEAS
\E [d^4(x_{n+1},x_\star) \vert\mathcal F_{n}]
&\leq&
 d^4(x_{n},x_\star) +2(2+\zeta)\gamma_{n+1}^2 \E [ \Vert \nabla f_{n+1}(x_n)\Vert^2 \vert\mathcal F_{n}]d^2(x_{n},x_\star) \\
 &&  +\gamma_{n+1}^4 \zeta^2 \E[ \Vert  \nabla f_{n+1}(x_n) \Vert^4  \vert\mathcal F_{n}] +4 \gamma_{n+1}\langle \nabla f(x_n),\Exp_{x_n}^{-1}(x_\star)\rangle d^2(x_{n},x_\star)  \\
 &&+ 4 \gamma_{n+1}^3 \zeta \E \Vert  \nabla f_{n+1}(x_n) \Vert^3 \vert\mathcal F_{n}] d(x_{n},x_\star).
\EEAS
Using that $f$ is g-strongly convex (Assumption~\ref{assump:strongconv}), the 4th-moment bound in Assumption~\ref{assump:noiseLip}, and Jensen's inequality we obtain,
\begin{multline*}
\E [d^4(x_{n+1},x_\star) \vert\mathcal F_{n}]\leq  (1-4\gamma_{n+1}\mu)d^4(x_{n},x_\star) +2(2+\zeta)\gamma_{n+1}^2 d^2(x_{n},x_\star) \upsilon^2 \\ +\gamma_{n+1}^4 \zeta^2 \upsilon^4 + 4 \gamma_{n+1}^3 \zeta \upsilon^3 d(x_{n},x_\star).
\end{multline*}
Using the upper bound $4 \gamma_{n+1}^3 \zeta \upsilon^3 d(x_{n},x_\star)  \leq 2 \gamma_{n+1}^4 \zeta^2 \upsilon^4+2  \gamma_{n+1}^2 \upsilon^2d(x_{n},x_\star) ^2 $, we have,
\begin{equation}\label{eq:dada}
\E [d^4(x_{n+1},x_\star) \vert\mathcal F_{n}]\leq  (1-4\gamma_{n+1}\mu)d^4(x_{n},x_\star) +2(3+\zeta)\upsilon^2\gamma_{n+1}^2 d^2(x_{n},x_\star)  +3\gamma_{n+1}^4 \zeta^2 \upsilon^4.
\end{equation}
Now let us define, $a_n= \E [d^4(x_{n+1},x_\star)]$,  $b_n= \E [d^2(x_{n+1},x_\star)]$ and  $u_n=a_n+\frac{2(3+\zeta)\upsilon^2}{\mu} \gamma_{n+1}b_n$. Taking the full expectation of \eq{dada}, we can bound $u_{n+1}$ as,
\BEAS
u_{n+1} &\leq &   (1-\gamma_{n+1}\mu) u_n  +3\gamma_{n+1}^4 \zeta^2 \upsilon^4 +\frac{2(3+\zeta)\zeta\upsilon^4}{\mu} \gamma_{n+1}^3 +2(3+\zeta)\upsilon^2\gamma_{n+1}^2 b_n\\
&&   -  (1-\gamma_{n+1}\mu) \frac{2(3+\zeta)\upsilon^2}{\mu} \gamma_{n+1} b_n+(1-2\gamma_{n+1}\mu) \frac{2(3+\zeta)\upsilon^2}{\mu} \gamma_{n+1} b_n.
\EEAS
Noting that $2(3+\zeta)\upsilon^2\gamma_{n+1}^2 b_n
   -  (1-\gamma_{n+1}\mu) \frac{2(3+\zeta)\upsilon^2}{\mu} \gamma_{n+1} b_n+(1-2\gamma_{n+1}\mu) \frac{2(3+\zeta)\upsilon^2}{\mu} \gamma_{n+1} b_n=0$, we obtain the simple upper-bound on $u_{n+1}$,
\[
u_{n+1} \leq    (1-\gamma_{n+1}\mu) u_n  +3\gamma_{n+1}^4 \zeta^2 \upsilon^4 +\frac{2(3+\zeta)\zeta\upsilon^4}{\mu} \gamma_{n+1}^3.
\]
Using $(1-x)\leq \exp( -x)$ for $x\in\mathbb R$, we have,
\[
u_{n+1} \leq   \exp (-\gamma_{n+1}\mu) u_n  +3\gamma_{n+1}^4 \zeta^2 \upsilon^4 +\frac{2(3+\zeta)\zeta\upsilon^4}{\mu} \gamma_{n+1}^3.
\]
We can unroll this recursion as before,
\[
u_{n} \leq   \exp (-\mu \sum_{i=1}^n \gamma_{i}) u_0  + \sum_{i=1}^n[3\zeta^2 \upsilon^4\gamma_{i}^4 +\frac{2(3+\zeta)\zeta\upsilon^4}{\mu} \gamma_{i}^3] \prod_{k=i+1}^n\exp(-\mu\gamma_k).
\]
Proceeding exactly as in the proof of the bound on the second moment, we may bound $u_n$ as
\[ u_n\leq \frac{2(3+\zeta)\zeta\upsilon^4}{\mu} \gamma_{\lfloor \frac{n}{2}\rfloor}^2 +\text{exponentially small  remainder terms}. \]
The conclusion follows.
\end{proof}
