\subsection{Proof of Proposition~\ref{prop:unknown}}

We first present a simpler helper lemma that will be used in the proof. 
One can view $X$ in the following lemma as a perturbation. The lemma bounds the effect of the perturbation to the left hand side of equation~\eqref{eqn:14}. 
\begin{lem}\label{lem:projection_change}
	Let $S \in \Real^{d \times r}$ be a column orthonormal matrix and
	$S^{\bot} = \Id - SS^{\top}$ be its orthogonal complement.
	Let $X \in \Real^{d\times d}$ be any matrix where $\norm{X} < \frac{1}{3}$.
	We have:
	\begin{align}
	\norm{\Id_{(\Id - X) S} (\Id - X) S^{\bot} + 2\Id_S X S^{\bot}}
	\lesssim \norm{X}^2. \label{eqn:14}
	\end{align} 	
\end{lem}

\begin{proof}
	By definition, we know that:
	\begin{align}
		\Id_{(\Id - X) S} &= (\Id - X) S \left( S^{\top}(\Id - X)^{\top} (\Id - X) S \right)^{-1}  S^{\top}(\Id - X)^{\top}	\nonumber \\
		&= (\Id - X) S \left(\Id - S^{\top} (X^{\top}  + X) S  + S^{\top} X^{\top} X S \right)^{-1} S^{\top}(\Id - X)^{\top} \label{eq_reduction}
	\end{align}
	Denote by $Y = S^{\top} (X^{\top} + X) S - S^{\top} X^{\top} X S$.
	We have that $\norm{Y}\le 2 \norm{X} + \norm{X}^2 < 7 \norm{X} / 3 $.
	By expanding $(\Id - Y)^{-1}$, we obtain:
	\begin{align*}
		\bignorm{(\Id - Y)^{-1} - (\Id + Y)}
		&\le \sum_{i=2}^{\infty} \norm{Y}^i \\
		&\le \frac {\norm{Y}^2} {1 - \norm{Y}} \le 25 \norm{X}^2.
	\end{align*}
	Hence we get:
	\[ \bignorm{(\Id - Y)^{-1} - (\Id + S^{\top} (X^{\top} + X) S)} \le 26 \norm{X}^2. \]
	Denote by
	\begin{align*}
		A &= (\Id - X) S \left(\Id + S^{\top} (X^{\top} + X) S\right) S^{\top} (\Id - X^{\top}) \\
			&= (\Id - X) \left(\Id_S + \Id_S (X^{\top} + X) \Id_S\right) (\Id - X^{\top}).
	\end{align*}
	We separate the terms in $A$ which has degree 1 in $X$:
	\begin{align*}
		A_1 &= \Id_S - X \Id_S - \Id_S X^{\top} + \Id_S (X^{\top} + X) \Id_S
	\end{align*}
	Consider the spectral norm of $A (\Id - X) S^{\bot}$.
	We have that $A_1 S^{\bot} = -\Id_S X S^{\bot}$.
	For $- A_1 X S^{\bot}$, the only term which has degree 1 in $X$ is $-\Id_S X S^{\bot}$.
	To summarize, we obtain by triangle inequality that:
	\begin{align*}
		\norm{\Id_{(\Id - X) S} (\Id - X) S^{\top} + 2\Id_S X S^{\bot}}
		&\le \norm{A + 2\Id_S X S^{\bot}} + 26 \norm{X}^2 \\
		&\lesssim \norm{A_1 + 2\Id_S X S^{\bot}} + \norm{X}^2 \lesssim \norm{X}^2
	\end{align*}
\end{proof}

\noindent Now we are ready present the proof of Proposition \ref{prop:unknown}.

\begin{proof}[Proof of Proposition~\ref{prop:unknown}]
	We first consider the term $\bM_t Z_t$:
	\begin{align}
		\bM_t \bZ_t &= \frac{1}{m}\sum_{i = 1}^m \langle \bA_i, \bU_t \bU_t^{\top} - \bXg \rangle \bA_i \bZ_t \nonumber
		\\
		& = \frac{1}{m}\sum_{i = 1}^m \left\langle \bA_i, Z_t Z_t^{\top} -\bXg\right\rangle   \bA_i \bZ_t 	\nonumber\\
		& + \frac{1}{m}  \sum_{i = 1}^m \left\langle \bA_i, \bE_t Z_t^{\top} + Z_t \bE_t^{\top}\right\rangle   \bA_iZ_t +  \frac{1}{m}\sum_{i = 1}^m \left\langle \bA_i,  \bE_t \bE_t^{\top}\right\rangle \bA_i \bZ_t  \label{eqn:15}
	\end{align}
	Note that $\nabla f(Z_t) =  \frac{1}{m}\sum_{i = 1}^m \left\langle \bA_i, Z_t Z_t^{\top} -\bXg\right\rangle   \bA_i \bZ_t$. 
	Using  Lemma~\ref{lem:property_1} and~\ref{lem:property_2} on the two terms in line~\eqref{eqn:15} with the fact that $Z_t^{\top} E_t = 0$, we have that
	\begin{align}
		&\left\|M_tZ_t - E_t Z_t^{\top} Z_t - \cG(Z_t)\right\|  \leq 
	2 \sqrt{r} \delta\| \bE_t\|\| Z_t\|^2 +  \delta d \| \bE_t \|^2 \|Z_t \|
		\label{eq_MtZt}
	\end{align}
We decompose $Z_{t+1}$ by: 
	\begin{align}
	Z_{t + 1} &= \Id_{S_{t + 1}} U_{t + 1} = U_{t + 1} - (\Id - \Id_{S_{t + 1}}) U_{t + 1} \nonumber
	\\
	& = (\Id - \eta M_{t }) Z_t + \left(\Id - \eta M_t \right) \bE_t  -  (\Id - \Id_{S_{t + 1}})  \left(\Id - \eta M_t \right) \bE_t  \nonumber
	\\
	&=  Z_t - \eta M_{t } Z_t  + \Id_{S_{t + 1}} ( \Id - \eta M_t ) E_t, \label{eq_Z_t+1}
	\end{align}
	where in the second equation we use the fact that
	$(\Id - \Id_{S_{t+1}}) (\Id - \eta M_t) Z_t = 0$,
	since the column subspace of $Z_t$ is $S_t$.
	Setting $S = \Id_{S_t}$ and $X = \eta M_t$ in Lemma \ref{lem:projection_change}, 
	we have that $\Id_{S_{t+1}} = \Id_{(\Id - X) S}$. Applying Lemma \ref{lem:projection_change}, we conclude:
	\begin{align*}
		\norm{\Id_{S_{t+1}} (\Id - \eta M_t) S^{\bot} + 2\Id_S (\Id - \eta M_t) S^{\bot}} \le \eta^2 \norm{M_t}^2,
	\end{align*}
	which implies that:
	\begin{align*}
		\norm{\Id_{S_{t+1}} (\Id - \eta M_t) E_t + 2\Id_S (\Id - \eta M_t) E_t} \le \eta^2 \norm{E_t} \norm{M_t}^2.
	\end{align*}
	Since $\norm{M_t} \le O(1)$ by Lemma \ref{lem_Mt},
	the conclusion follows by combining Equation \eqref{eq_MtZt} and \eqref{eq_Z_t+1} with the equation above.
\end{proof}

